verified/entry.s.dfy
@@ -1,7 +1,5 @@
-include "kom_common.s.dfy"
 include "ARMdef.dfy"
 include "pagedb.s.dfy"
-include "smcapi.s.dfy"
 include "abstate.s.dfy"
 
 predicate nonStoppedL1(d:PageDb, l1:PageNr)
@@ -23,8 +21,23 @@ function l1pOfDispatcher(d:PageDb, p:PageNr) : PageNr
     d[d[p].addrspace].entry.l1ptnr
 }
 
+// common success/failure checks for enter and resume
+function smc_enter_err(d: PageDb, p: word, isresume: bool): word
+    requires validPageDb(d)
+{
+    reveal_validPageDb();
+    if (!(validPageNr(p) && d[p].PageDbEntryTyped? && d[p].entry.Dispatcher?)) then
+        KOM_ERR_INVALID_PAGENO()
+    else if (var a := d[p].addrspace; d[a].entry.state != FinalState) then
+        KOM_ERR_NOT_FINAL()
+    else if (!isresume && d[p].entry.entered) then
+        KOM_ERR_ALREADY_ENTERED()
+    else if (isresume && !d[p].entry.entered) then
+        KOM_ERR_NOT_ENTERED()
+    else KOM_ERR_SUCCESS()
+}
 
-// This must hold between all consecutive states on the addsrpace entry/return path.
+// This must hold between all consecutive states on the addsrpace entry/resume path.
 predicate validERTransition(s:SysState, s':SysState, dispPg:PageNr)
     requires validDispatcherPage(s.d, dispPg)
 {
@@ -34,7 +47,6 @@ predicate validERTransition(s:SysState, s':SysState, dispPg:PageNr)
     && equivalentExceptPage(s.d, s'.d, dispPg)
     && nonStoppedDispatcher(s.d, dispPg) && nonStoppedDispatcher(s'.d, dispPg)
     && page_paddr(l1pOfDispatcher(s.d, dispPg))  == s.hw.conf.ttbr0.ptbase
-    && s.hw.conf.ttbr0.ptbase == s'.hw.conf.ttbr0.ptbase
     && WSMemInvariantExceptAddrspaceAtPage(s.hw, s'.hw, s.d,
         l1pOfDispatcher(s.d, dispPg)))
 }
@@ -55,148 +67,156 @@ predicate validERTransitionHW(hw:state, hw':state, d:PageDb)
     ValidState(hw) && ValidState(hw') && hw'.conf.ttbr0 == hw.conf.ttbr0
     && physPageIsSecure(hw.conf.ttbr0.ptbase / PAGESIZE())
     && nonStoppedL1(d, securePageFromPhysAddr(hw.conf.ttbr0.ptbase))
-    //&& bankedRegsPreserved(hw, hw')
-}
-
-predicate validSysStates(sset:set<SysState>) { forall s :: s in sset ==> validSysState(s) }
-
-// This is just here to make verification easier. It allows irrelevant state 
-// (i.e. some regs) to be changed while checking for error conditions.
-predicate errCheck(s:SysState, s':SysState)
-{
-   validSysState(s) && validSysState(s') && s.d == s'.d
 }
 
 predicate validEnter(s:SysState,s':SysState,
-    dispPage:word,a1:word,a2:word,a3:word)
+    dispPg:word,a1:word,a2:word,a3:word)
     requires validSysState(s)
-    // requires smc_enter(s.d, dispPage, a1, a2, a3).1 == KOM_ERR_SUCCESS()
+    requires smc_enter_err(s.d, dispPg, false) == KOM_ERR_SUCCESS()
 {
     reveal_ValidRegState();
     reveal_validExceptionTransition();
-    smc_enter(s.d, dispPage, a1, a2, a3).1 != KOM_ERR_SUCCESS() ||
-   
-    ((exists serr, s2, s3, s4 :: validSysStates({serr,s2,s3,s4})
-        && errCheck(s, serr)
-        && preEntryEnter(serr,s2,dispPage,a1,a2,a3)
-        && entryTransitionEnter(s2, s3, dispPage)
-        && s4.d == s3.d && userspaceExecution(s3.hw, s4.hw, s3.d)
-        && mode_of_state(s4.hw) != User
-        && validExceptionTransition(s4, s', dispPage)
-        && (s'.hw.regs[R0], s'.hw.regs[R1], s'.d)==
-            exceptionHandled(s4, dispPage))
-    && bankedRegsPreserved(s.hw, s'.hw))
+    exists s2, s3, s4 | ValidState(s2) && ValidState(s3) && ValidState(s4) ::
+        preEntryEnter(s.hw, s2, s.d, dispPg, a1, a2, a3)
+        && entryTransitionEnter(s2, s3, s.d, dispPg)
+        && userspaceExecution(s3, s4, s.d)
+        && mode_of_state(s4) != User
+        && validExceptionTransition(SysState(s4, s.d), s', dispPg)
+        && (s'.hw.regs[R0], s'.hw.regs[R1], s'.d) ==
+            exceptionHandled(s4, s.d, dispPg)
 }
 
 predicate validResume(s:SysState,s':SysState,dispPg:word)
     requires validSysState(s)
+    requires smc_enter_err(s.d, dispPg, true) == KOM_ERR_SUCCESS()
 {
      
     reveal_ValidRegState();
     reveal_validExceptionTransition();
-    smc_resume(s.d, dispPg).1 != KOM_ERR_SUCCESS() ||
-   
-    ((exists serr, s2, s3, s4 :: validSysStates({serr,s2,s3,s4})
-        && errCheck(s, serr)
-        && preEntryResume(serr,s2,dispPg)
-        && entryTransitionResume(s2, s3, dispPg)
-        && s4.d == s3.d && userspaceExecution(s3.hw, s4.hw, s3.d)
-        && mode_of_state(s4.hw) != User
-        && validExceptionTransition(s4, s', dispPg)
+    exists s2, s3, s4 | ValidState(s2) && ValidState(s3) && ValidState(s4) ::
+        preEntryResume(s.hw, s2, s.d, dispPg)
+        && entryTransitionResume(s2, s3, s.d, dispPg)
+        && userspaceExecution(s3, s4, s.d)
+        && mode_of_state(s4) != User
+        && validExceptionTransition(SysState(s4, s.d), s', dispPg)
         && (s'.hw.regs[R0], s'.hw.regs[R1], s'.d)==
-            exceptionHandled(s4, dispPg))
-    && bankedRegsPreserved(s.hw, s'.hw))
+            exceptionHandled(s4, s.d, dispPg)
 }
 
-predicate preEntryEnter(s:SysState,s':SysState,
+predicate smc_enter(s: state, pageDbIn: PageDb, s':state, pageDbOut: PageDb,
+                    dispPage: word, arg1: word, arg2: word, arg3: word)
+    requires ValidState(s) && validPageDb(pageDbIn) && ValidState(s')
+{
+    reveal_ValidRegState();
+    var err := smc_enter_err(pageDbIn, dispPage, false);
+    if err != KOM_ERR_SUCCESS() then
+        pageDbOut == pageDbIn && s'.regs[R0] == err && s'.regs[R1] == 0
+    else
+        validEnter(SysState(s, pageDbIn), SysState(s', pageDbOut), dispPage,
+                   arg1, arg2, arg3)
+}
+
+predicate smc_resume(s: state, pageDbIn: PageDb, s':state, pageDbOut: PageDb,
+                     dispPage: word)
+    requires ValidState(s) && validPageDb(pageDbIn) && ValidState(s')
+{
+    reveal_ValidRegState();
+    var err := smc_enter_err(pageDbIn, dispPage, true);
+    if err != KOM_ERR_SUCCESS() then
+        pageDbOut == pageDbIn && s'.regs[R0] == err && s'.regs[R1] == 0
+    else
+        validResume(SysState(s, pageDbIn), SysState(s', pageDbOut), dispPage)
+}
+
+predicate preEntryEnter(s:state,s':state,d:PageDb,
     dispPage:PageNr,a1:word,a2:word,a3:word)
-    requires validSysState(s)
-    requires smc_enter(s.d, dispPage, a1, a2, a3).1 == KOM_ERR_SUCCESS()
-    ensures preEntryEnter(s,s',dispPage,a1,a2,a3) ==>
-        PageAligned(s'.hw.conf.ttbr0.ptbase) &&
-        SecurePhysBase() <= s'.hw.conf.ttbr0.ptbase < SecurePhysBase() +
+    requires ValidState(s)
+    requires validPageDb(d)
+    requires smc_enter_err(d, dispPage, false) == KOM_ERR_SUCCESS()
+    ensures preEntryEnter(s,s',d,dispPage,a1,a2,a3) ==>
+        PageAligned(s'.conf.ttbr0.ptbase) &&
+        SecurePhysBase() <= s'.conf.ttbr0.ptbase < SecurePhysBase() +
             KOM_SECURE_NPAGES() * PAGESIZE()
-    ensures preEntryEnter(s,s',dispPage,a1,a2,a3) ==>
-        nonStoppedL1(s'.d, securePageFromPhysAddr(s'.hw.conf.ttbr0.ptbase));
+    ensures preEntryEnter(s,s',d,dispPage,a1,a2,a3) ==>
+        nonStoppedL1(d, securePageFromPhysAddr(s'.conf.ttbr0.ptbase));
 {
     reveal_validPageDb();
     reveal_ValidRegState();
-    var addrspace := s.d[s.d[dispPage].addrspace];
-    assert isAddrspace(s.d, s.d[dispPage].addrspace);
+    var addrspace := d[d[dispPage].addrspace];
+    assert isAddrspace(d, d[dispPage].addrspace);
     var l1p := addrspace.entry.l1ptnr; // l1pOfDispatcher(s.d, dispPage);
-    assert s.d[l1p].addrspace == s.d[dispPage].addrspace;
+    assert d[l1p].addrspace == d[dispPage].addrspace;
     assert addrspace.entry.state == FinalState;
-    assert !hasStoppedAddrspace(s.d, l1p);
+    assert !hasStoppedAddrspace(d, l1p);
 
-    validSysState(s') &&  s.d == s'.d &&
-    s'.hw.conf.ttbr0.ptbase == page_paddr(l1p) &&
-    s'.hw.conf.scr.ns == Secure &&
-    s'.hw.regs[R0] == a1 && s'.hw.regs[R1] == a2 && s'.hw.regs[R2] == a3 &&
+    ValidState(s') &&
+    s'.conf.ttbr0.ptbase == page_paddr(l1p) &&
+    s'.conf.scr.ns == Secure &&
+    s'.regs[R0] == a1 && s'.regs[R1] == a2 && s'.regs[R2] == a3 &&
 
-    WSMemInvariantExceptAddrspaceAtPage(s.hw, s'.hw, s.d, l1p)
+    WSMemInvariantExceptAddrspaceAtPage(s, s', d, l1p)
 }
 
-predicate preEntryResume(s:SysState, s':SysState, dispPage:PageNr)
-    requires validSysState(s)
-    requires smc_resume(s.d, dispPage).1 == KOM_ERR_SUCCESS()
-    ensures preEntryResume(s,s',dispPage) ==>
-        PageAligned(s'.hw.conf.ttbr0.ptbase) &&
-        SecurePhysBase() <= s'.hw.conf.ttbr0.ptbase < SecurePhysBase() +
+predicate preEntryResume(s:state, s':state, d:PageDb, dispPage:PageNr)
+    requires ValidState(s) && validPageDb(d)
+    requires smc_enter_err(d, dispPage, true) == KOM_ERR_SUCCESS()
+    ensures preEntryResume(s,s',d,dispPage) ==>
+        PageAligned(s'.conf.ttbr0.ptbase) &&
+        SecurePhysBase() <= s'.conf.ttbr0.ptbase < SecurePhysBase() +
             KOM_SECURE_NPAGES() * PAGESIZE()
-    ensures preEntryResume(s,s',dispPage) ==>
-        nonStoppedL1(s'.d, securePageFromPhysAddr(s'.hw.conf.ttbr0.ptbase));
+    ensures preEntryResume(s,s',d,dispPage) ==>
+        nonStoppedL1(d, securePageFromPhysAddr(s'.conf.ttbr0.ptbase));
 {
     reveal_validPageDb();
-    var disp := s.d[dispPage].entry;
-    var l1p := l1pOfDispatcher(s.d, dispPage);
+    var disp := d[dispPage].entry;
+    var l1p := l1pOfDispatcher(d, dispPage);
     
-    validSysState(s') && s'.d == s.d &&
-    s'.hw.conf.ttbr0.ptbase == page_paddr(l1p) && //l1pOfDispatcher(s.d, dispPage) &&
-    s'.hw.conf.scr.ns == Secure &&
+    ValidState(s') &&
+    s'.conf.ttbr0.ptbase == page_paddr(l1p) && //l1pOfDispatcher(d, dispPage) &&
+    s'.conf.scr.ns == Secure &&
 
     (reveal_ValidRegState(); 
-    s'.hw.regs[R0] == disp.ctxt.regs[R0] &&
-    s'.hw.regs[R1] == disp.ctxt.regs[R1] &&
-    s'.hw.regs[R2] == disp.ctxt.regs[R2] &&
-    s'.hw.regs[R3] == disp.ctxt.regs[R3] &&
-    s'.hw.regs[R4] == disp.ctxt.regs[R4] &&
-    s'.hw.regs[R5] == disp.ctxt.regs[R5] &&
-    s'.hw.regs[R6] == disp.ctxt.regs[R6] &&
-    s'.hw.regs[R7] == disp.ctxt.regs[R7] &&
-    s'.hw.regs[R8] == disp.ctxt.regs[R8] &&
-    s'.hw.regs[R9] == disp.ctxt.regs[R9] &&
-    s'.hw.regs[R10] == disp.ctxt.regs[R10] &&
-    s'.hw.regs[R11] == disp.ctxt.regs[R11] &&
-    s'.hw.regs[R12] == disp.ctxt.regs[R12] &&
-    s'.hw.regs[LR(User)] == disp.ctxt.regs[LR(User)] &&
-    s'.hw.regs[SP(User)] == disp.ctxt.regs[SP(User)]) &&
+    s'.regs[R0] == disp.ctxt.regs[R0] &&
+    s'.regs[R1] == disp.ctxt.regs[R1] &&
+    s'.regs[R2] == disp.ctxt.regs[R2] &&
+    s'.regs[R3] == disp.ctxt.regs[R3] &&
+    s'.regs[R4] == disp.ctxt.regs[R4] &&
+    s'.regs[R5] == disp.ctxt.regs[R5] &&
+    s'.regs[R6] == disp.ctxt.regs[R6] &&
+    s'.regs[R7] == disp.ctxt.regs[R7] &&
+    s'.regs[R8] == disp.ctxt.regs[R8] &&
+    s'.regs[R9] == disp.ctxt.regs[R9] &&
+    s'.regs[R10] == disp.ctxt.regs[R10] &&
+    s'.regs[R11] == disp.ctxt.regs[R11] &&
+    s'.regs[R12] == disp.ctxt.regs[R12] &&
+    s'.regs[LR(User)] == disp.ctxt.regs[LR(User)] &&
+    s'.regs[SP(User)] == disp.ctxt.regs[SP(User)]) &&
     
     (reveal_ValidSRegState();
-    s'.hw.sregs[spsr(Monitor)] == disp.ctxt.cpsr) &&
-    //s'.hw.conf.cpsr == decode_psr(disp.ctxt.cpsr)) &&
+    s'.sregs[spsr(Monitor)] == disp.ctxt.cpsr) &&
+    //s'.conf.cpsr == decode_psr(disp.ctxt.cpsr)) &&
     
-    WSMemInvariantExceptAddrspaceAtPage(s.hw, s'.hw, s.d, l1p)
-
+    WSMemInvariantExceptAddrspaceAtPage(s, s', d, l1p)
 }
 
-predicate entryTransitionEnter(s:SysState, s':SysState, dispPg:PageNr)
-    requires validDispatcherPage(s.d, dispPg)
-    ensures entryTransitionEnter(s, s', dispPg) ==> mode_of_state(s'.hw) == User
+predicate entryTransitionEnter(s:state, s':state, d:PageDb, dispPg:PageNr)
+    requires validDispatcherPage(d, dispPg)
+    ensures entryTransitionEnter(s, s', d, dispPg) ==> mode_of_state(s') == User
 {
-    validERTransition(s, s', dispPg) && s'.d == s.d
-    && evalEnterUserspace(s.hw, s'.hw)
-    && s'.hw.steps == s.hw.steps + 1
-    && OperandContents(s.hw, OLR) == s.d[dispPg].entry.entrypoint
+    validERTransition(SysState(s,d), SysState(s',d), dispPg)
+    && evalEnterUserspace(s, s')
+    && s'.steps == s.steps + 1
+    && OperandContents(s, OLR) == d[dispPg].entry.entrypoint
 }
 
-predicate entryTransitionResume(s:SysState, s':SysState, dispPg:PageNr)
-    requires validDispatcherPage(s.d, dispPg)
+predicate entryTransitionResume(s:state, s':state, d:PageDb, dispPg:PageNr)
+    requires validDispatcherPage(d, dispPg)
 {
-    validSysState(s) && validSysState(s') && s.d == s'.d
-    && evalEnterUserspace(s.hw, s'.hw)
-    && s'.hw.steps == s.hw.steps + 1
-    && (var disp := s.d[dispPg].entry;
-    OperandContents(s.hw, OLR) == disp.ctxt.pc)
+    ValidState(s) && ValidState(s')
+    && evalEnterUserspace(s, s')
+    && s'.steps == s.steps + 1
+    && (var disp := d[dispPg].entry;
+    OperandContents(s, OLR) == disp.ctxt.pc)
 }
 
 predicate userspaceExecution(hw:state, hw':state, d:PageDb)
@@ -216,42 +236,42 @@ predicate userspaceExecution(hw:state, hw':state, d:PageDb)
 //-----------------------------------------------------------------------------
 // Exception Handler Spec
 //-----------------------------------------------------------------------------
-function exceptionHandled(s:SysState, dispPg:PageNr) : (word, word, PageDb)
-    requires validSysState(s)
-    requires mode_of_state(s.hw) != User
-    requires validDispatcherPage(s.d, dispPg)
+function exceptionHandled(s:state, d:PageDb, dispPg:PageNr) : (word, word, PageDb)
+    requires ValidState(s) && validPageDb(d)
+    requires mode_of_state(s) != User
+    requires validDispatcherPage(d, dispPg)
     // This should be true since the exception is taken from user mode
     requires 
         (reveal_ValidSRegState();
         decode_mode'(psr_mask_mode(
-        s.hw.sregs[spsr(mode_of_state(s.hw))])) == Just(User))
-    ensures var (r0,r1,d') := exceptionHandled(s, dispPg);
+        s.sregs[spsr(mode_of_state(s))])) == Just(User))
+    ensures var (r0,r1,d') := exceptionHandled(s, d, dispPg);
         wellFormedPageDb(d')
 {
     reveal_validPageDb();
     reveal_ValidSRegState();
     reveal_ValidRegState();
-    if(s.hw.conf.ex.ExSVC?) then
+    if(s.conf.ex.ExSVC?) then
         var p := dispPg;
-        var d' := s.d[ p := s.d[p].(entry := s.d[p].entry.(entered := false))];
-        (KOM_ERR_SUCCESS(), s.hw.regs[R0], d')
+        var d' := d[ p := d[p].(entry := d[p].entry.(entered := false))];
+        (KOM_ERR_SUCCESS(), s.regs[R0], d')
     else 
         var p := dispPg;
-        var pc := OperandContents(s.hw, OLR);
-        var psr := s.hw.sregs[spsr(mode_of_state(s.hw))];
+        var pc := OperandContents(s, OLR);
+        var psr := s.sregs[spsr(mode_of_state(s))];
         assert decode_mode'(psr_mask_mode(psr)) == Just(User);
-        var ctxt' := DispatcherContext(s.hw.regs, pc, psr);
+        var ctxt' := DispatcherContext(s.regs, pc, psr);
         assert decode_mode'(psr_mask_mode(ctxt'.cpsr)) == Just(User);
         assert validDispatcherContext(ctxt');
-        var disp' := s.d[p].entry.(entered:=true, ctxt:=ctxt');
-        var d' := s.d[ p := s.d[p].(entry := disp') ];
-        assert wellFormedPageDbEntry(s.d[p].(entry := disp'));
+        var disp' := d[p].entry.(entered:=true, ctxt:=ctxt');
+        var d' := d[ p := d[p].(entry := disp') ];
+        assert wellFormedPageDbEntry(d[p].(entry := disp'));
         assert wellFormedPageDb(d');
-        if s.hw.conf.ex.ExIRQ? || s.hw.conf.ex.ExFIQ? then
+        if s.conf.ex.ExIRQ? || s.conf.ex.ExFIQ? then
             (KOM_ERR_INTERRUPTED(), 0, d')
         else
-            assert s.hw.conf.ex.ExAbt? || s.hw.conf.ex.ExUnd? ||
-                s.hw.conf.ex.ExUnd?;
+            assert s.conf.ex.ExAbt? || s.conf.ex.ExUnd? ||
+                s.conf.ex.ExUnd?;
             (KOM_ERR_FAULT(), 0, d')
 }
 
@@ -265,17 +285,13 @@ predicate {:opaque} validExceptionTransition(s:SysState, s':SysState, dispPg: Pa
     reveal_ValidMemState();
     validSysState(s) && validSysState(s') &&
     (validERTransitionHW(s.hw, s'.hw, s.d)
-    && equivalentExceptPage(s.d, s'.d, dispPg) 
+    && equivalentExceptPage(s.d, s'.d, dispPg)
     && nonStoppedDispatcher(s.d, dispPg) && nonStoppedDispatcher(s'.d, dispPg)
     && page_paddr(l1pOfDispatcher(s.d, dispPg)) == s.hw.conf.ttbr0.ptbase
-    && s.hw.conf.ttbr0.ptbase == s'.hw.conf.ttbr0.ptbase  
-    // && (forall g | ValidGlobal(g) && g != PageDb() ::
-    //    GlobalFullContents(s.hw.m, g) == GlobalFullContents(s'.hw.m, g))
-    && (forall p:PageNr | p != dispPg :: s.d[p] == s'.d[p])
-        //extractPageDbEntry(s.hw.m, p) == extractPageDbEntry(s'.hw.m, p))
-    && (forall a:addr | a in TheValidAddresses() && !(StackLimit() <= a < StackBase()) && 
+    && s.hw.conf.ttbr0.ptbase == s'.hw.conf.ttbr0.ptbase
+    && (forall a:addr | a in TheValidAddresses() && !(StackLimit() <= a < StackBase()) &&
         !(addrInPage(a, dispPg)) :: s.hw.m.addresses[a] == s'.hw.m.addresses[a])
-    && mode_of_state(s.hw) != User 
+    && mode_of_state(s.hw) != User
     && mode_of_state(s'.hw) == Monitor)
 }
 
