verified/abstate.s.dfy
@@ -1,10 +1,9 @@
-include "pagedb.s.dfy"
 include "ARMdef.dfy"
-include "kom_common.s.dfy"
+include "pagedb.s.dfy"
 
 datatype SysState = SysState(hw:state, d:PageDb)
 
 predicate validSysState(s:SysState)
 {
-    ValidState(s.hw) /*&& SaneMem(s.hw.m)*/ && validPageDb(s.d)
+    ValidState(s.hw) && validPageDb(s.d)
 }
